src/lib/communication/DY.Lib.Communication.API.fst
@@ -10,15 +10,37 @@ open DY.Lib.Event.Typed
 
 (*** Messages ***)
 
+
 [@@with_bytes bytes]
-type communication_message = {
+type communication_message_base = {
   sender:principal;
   receiver:principal;  
   payload:bytes;
 }
 
+%splice [ps_communication_message_base] (gen_parser (`communication_message_base))
+%splice [ps_communication_message_base_is_well_formed] (gen_is_well_formed_lemma (`communication_message_base))
+
+[@@with_bytes bytes]
+type communication_message_sign = {
+  sender:principal;
+  receiver:principal;  
+  payload:bytes;
+  signature:bytes;
+}
+
+%splice [ps_communication_message_sign] (gen_parser (`communication_message_sign))
+%splice [ps_communication_message_sign_is_well_formed] (gen_is_well_formed_lemma (`communication_message_sign))
+
+[@@with_bytes bytes]
+type communication_message = 
+  | CM: msg:communication_message_base -> communication_message
+  | CMSign: msg:communication_message_sign -> communication_message
+
+#push-options "--ifuel 1 --fuel 0"
 %splice [ps_communication_message] (gen_parser (`communication_message))
 %splice [ps_communication_message_is_well_formed] (gen_is_well_formed_lemma (`communication_message))
+#pop-options
 
 instance parseable_serializeable_bytes_communication_message: parseable_serializeable bytes communication_message
   = mk_parseable_serializeable ps_communication_message
@@ -28,12 +50,14 @@ instance parseable_serializeable_bytes_communication_message: parseable_serializ
 #push-options "--ifuel 1 --fuel 0"
 [@@with_bytes bytes]
 type communication_event =
-  | CommunicationLayerSendMsg: sender:principal -> receiver:principal -> payload:bytes -> communication_event
-  | CommunicationLayerReceiveMsg: sender:principal -> receiver:principal -> payload:bytes -> communication_event
+  | CommConfSendMsg: sender:principal -> receiver:principal -> payload:bytes -> communication_event
+  | CommConfReceiveMsg: sender:principal -> receiver:principal -> payload:bytes -> communication_event
+  | CommAuthSendMsg: sender:principal -> payload:bytes -> communication_event
+  | CommAuthReceiveMsg: sender:principal -> receiver:principal -> vk_sender:bytes -> payload:bytes -> communication_event
 
 %splice [ps_communication_event] (gen_parser (`communication_event))
 %splice [ps_communication_event_is_well_formed] (gen_is_well_formed_lemma (`communication_event))
-
+#pop-options
 
 instance event_communication_event: event communication_event = {
   tag = "DY.Lib.Communication.Event";
@@ -42,8 +66,11 @@ instance event_communication_event: event communication_event = {
 
 (*** Layer Setup ***)
 
-val comm_layer_tag: string
-let comm_layer_tag = "DY.Lib.Communication.PublicKey"
+val comm_layer_pkenc_tag: string
+let comm_layer_pkenc_tag = "DY.Lib.Communication.PkEnc.PublicKey"
+
+val comm_layer_sign_tag: string
+let comm_layer_sign_tag = "DY.Lib.Communication.Sign.PublicKey"
 
 (*** Communication Layer ***)
 
@@ -57,20 +84,20 @@ type communication_keys_sess_ids = {
 val initialize_communication: principal -> principal -> traceful (option (communication_keys_sess_ids & communication_keys_sess_ids))
 let initialize_communication sender receiver =
   let* client_global_session_priv_key_id = initialize_private_keys sender in
-  generate_private_key sender client_global_session_priv_key_id (PkDec "DY.Lib.Communication.PublicKey");*
+  generate_private_key sender client_global_session_priv_key_id (PkDec comm_layer_pkenc_tag);*
 
   let* receiver_global_session_priv_key_id = initialize_private_keys receiver in
-  generate_private_key receiver receiver_global_session_priv_key_id (PkDec "DY.Lib.Communication.PublicKey");*
+  generate_private_key receiver receiver_global_session_priv_key_id (PkDec comm_layer_pkenc_tag);*
 
-  let*? priv_key_receiver = get_private_key receiver receiver_global_session_priv_key_id (PkDec "DY.Lib.Communication.PublicKey") in
+  let*? priv_key_receiver = get_private_key receiver receiver_global_session_priv_key_id (PkDec comm_layer_pkenc_tag) in
   let pub_key_receiver = pk priv_key_receiver in
   let* client_global_session_pub_key_id = initialize_pki sender in
-  install_public_key sender client_global_session_pub_key_id (PkEnc "DY.Lib.Communication.PublicKey") receiver pub_key_receiver;*
+  install_public_key sender client_global_session_pub_key_id (PkEnc comm_layer_pkenc_tag) receiver pub_key_receiver;*
 
-  let*? priv_key_client = get_private_key sender client_global_session_priv_key_id (PkDec "DY.Lib.Communication.PublicKey") in
+  let*? priv_key_client = get_private_key sender client_global_session_priv_key_id (PkDec comm_layer_pkenc_tag) in
   let pub_key_client = pk priv_key_client in
   let* receiver_global_session_pub_key_id = initialize_pki receiver in
-  install_public_key receiver receiver_global_session_pub_key_id (PkEnc "DY.Lib.Communication.PublicKey") sender pub_key_client;*
+  install_public_key receiver receiver_global_session_pub_key_id (PkEnc comm_layer_pkenc_tag) sender pub_key_client;*
 
   let client_comm_keys_sess_ids = {pki=client_global_session_pub_key_id; private_keys=client_global_session_priv_key_id} in
   let receiver_comm_keys_sess_ids = {pki=receiver_global_session_pub_key_id; private_keys=receiver_global_session_priv_key_id} in
@@ -81,7 +108,7 @@ let initialize_communication sender receiver =
 
 val encrypt_message: principal -> principal -> bytes -> bytes -> bytes -> bytes
 let encrypt_message sender receiver payload pk nonce =
-  let msg = {sender; receiver; payload} in
+  let msg = CM {sender; receiver; payload} in
   let msg_bytes = serialize communication_message msg in
   pk_enc pk nonce msg_bytes
 
@@ -89,29 +116,74 @@ val send_confidential:
   communication_keys_sess_ids ->
   principal -> principal -> bytes ->
   traceful (option timestamp)
-let send_confidential keys_sess_ids sender receiver payload =
-  let*? pk_receiver = get_public_key sender keys_sess_ids.pki (PkEnc "DY.Lib.Communication.PublicKey") receiver in
+let send_confidential comm_keys_ids sender receiver payload =
+  let*? pk_receiver = get_public_key sender comm_keys_ids.pki (PkEnc comm_layer_pkenc_tag) receiver in
   let* nonce = mk_rand PkNonce (principal_label sender) 32 in
+  trigger_event sender (CommConfSendMsg sender receiver payload);*
   let msg_encrypted = encrypt_message sender receiver payload pk_receiver nonce in
   let* msg_id = send_msg msg_encrypted in  
   return (Some msg_id)
 
 
-val decrypt_message: bytes -> bytes -> option communication_message
+val decrypt_message: bytes -> bytes -> option communication_message_base
 let decrypt_message sk_receiver msg_encrypted =
   let? msg_plain_bytes = pk_dec sk_receiver msg_encrypted in
   let? msg_plain = parse communication_message msg_plain_bytes in
-  Some msg_plain
+  guard(CM? msg_plain);?
+  Some (CM?.msg msg_plain)
 
 val receive_confidential:
   communication_keys_sess_ids ->
   principal -> timestamp ->
-  traceful (option communication_message)
-let receive_confidential keys_sess_ids receiver msg_id =
-  let*? sk_receiver = get_private_key receiver keys_sess_ids.private_keys (PkDec "DY.Lib.Communication.PublicKey") in
+  traceful (option communication_message_base)
+let receive_confidential comm_keys_ids receiver msg_id =
+  let*? sk_receiver = get_private_key receiver comm_keys_ids.private_keys (PkDec comm_layer_pkenc_tag) in
   let*? msg_encrypted = recv_msg msg_id in
-  let*? msg_plain:communication_message = return (decrypt_message sk_receiver msg_encrypted) in
+  let*? msg_plain:communication_message_base = return (decrypt_message sk_receiver msg_encrypted) in
+  trigger_event receiver (CommConfReceiveMsg msg_plain.sender receiver msg_plain.payload);*
   return (Some msg_plain)
 
 
-(**** Confidential and Authenticated Send and Receive Functions ****)
+(**** Authenticated Send and Receive Functions ****)
+
+val sign_message: principal -> principal -> bytes -> bytes -> bytes -> bytes
+let sign_message sender receiver payload sk nonce =
+  let msg = CM {sender; receiver; payload} in
+  let msg_bytes = serialize communication_message msg in
+  let signature = sign sk nonce msg_bytes in
+  let msg_signed = CMSign {sender; receiver; payload; signature} in
+  serialize communication_message msg_signed
+
+val send_authenticated:
+  communication_keys_sess_ids ->
+  principal -> principal -> bytes ->
+  traceful (option timestamp)
+let send_authenticated comm_keys_ids sender receiver payload =
+  let*? sk_sender = get_private_key sender comm_keys_ids.private_keys (Sign comm_layer_sign_tag) in
+  let* nonce = mk_rand SigNonce (principal_label sender) 32 in
+  trigger_event sender (CommAuthSendMsg sender payload);*
+  let msg_signed = sign_message sender receiver payload sk_sender nonce in
+  let* msg_id = send_msg msg_signed in
+  return (Some msg_id)
+
+
+val verify_message: principal -> bytes -> bytes -> option communication_message_base
+let verify_message receiver msg_bytes vk_sender =
+  let? cm_msg = parse communication_message msg_bytes in
+  guard (CMSign? cm_msg);?
+  let msg_signed = CMSign?.msg cm_msg in
+  let msg = CM {sender=msg_signed.sender; receiver=msg_signed.receiver; payload=msg_signed.payload} in
+  let msg_bytes = serialize communication_message (msg) in
+  guard (verify vk_sender msg_bytes msg_signed.signature);?
+  Some (CM?.msg msg)
+
+val receive_authenticated:
+  communication_keys_sess_ids ->
+  principal -> principal -> timestamp ->
+  traceful (option communication_message_base)
+let receive_authenticated comm_keys_ids sender receiver msg_id =
+  let*? vk_sender = get_public_key receiver comm_keys_ids.pki (Verify comm_layer_sign_tag) sender in
+  let*? msg_encrypted = recv_msg msg_id in
+  let*? msg_plain:communication_message_base = return (verify_message receiver msg_encrypted vk_sender) in
+  trigger_event receiver (CommAuthReceiveMsg sender receiver vk_sender msg_plain.payload);*
+  return (Some msg_plain)
